This change adds the Arm implementation of ML-DSA Forward NTT function and its HolLight proof of correctness. At this moment, the implementation is the same as the one in mlkem-native repository at https://github.com/pq-code-package/mlkem-native.
The proof was developed with the help of Anthropic Opus 4.6.

arm/proofs/subroutine_signatures.ml
@@ -4399,6 +4399,25 @@ let subroutine_signatures = [
    ])
 );
 
+("mldsa_ntt_arm",
+  ([(*args*)
+     ("a", "int32_t[static 256]", (*is const?*)"false");
+     ("z_012345", "int32_t[144]", (*is const?*)"true");
+     ("z_67", "int32_t[384]", (*is const?*)"true");
+   ],
+   "void",
+   [(* input buffers *)
+    ("a", "256"(* num elems *), 4(* elem bytesize *));
+    ("z_012345", "144"(* num elems *), 4(* elem bytesize *));
+    ("z_67", "384"(* num elems *), 4(* elem bytesize *));
+   ],
+   [(* output buffers *)
+    ("a", "256"(* num elems *), 4(* elem bytesize *));
+   ],
+   [(* temporary buffers *)
+   ])
+);
+
 ("mlkem_basemul_k2",
   ([(*args*)
      ("r", "int16_t[static 256]", (*is const?*)"false");
