benchmarks/benchmark.c
@@ -1121,7 +1121,7 @@ void call_sha3_keccak4_f1600_alt2(void) {}
 #else
 
 void call_mldsa_intt(void) {}
-void call_mldsa_ntt(void) {}
+void call_mldsa_ntt(void) repeat(mldsa_ntt_arm((int32_t*)b0,(const int32_t*)b1,(const int32_t*)b2))
 void call_mldsa_reduce(void) {}
 
 void call_bignum_copy_row_from_table_8n__32_16(void) \
@@ -1542,7 +1542,7 @@ int main(int argc, char *argv[])
   timingtest(all,"mlkem_tomont",call_mlkem_tomont);
   timingtest(!arm,"mlkem_unpack",call_mlkem_unpack);
   timingtest(!arm,"mldsa_intt",call_mldsa_intt);
-  timingtest(!arm,"mldsa_ntt",call_mldsa_ntt);
+  timingtest(all,"mldsa_ntt",call_mldsa_ntt);
   timingtest(!arm,"mldsa_reduce",call_mldsa_reduce);
   timingtest(bmi,"p256_montjadd",call_p256_montjadd);
   timingtest(all,"p256_montjadd_alt",call_p256_montjadd_alt);
